wip

src/localdrf/LocalDRFDef.v
@@ -1324,3 +1324,306 @@ Proof.
     des_ifs. ss. des; clarify.
     eapply Memory.remove_get0 in PROMISES. des. clarify.
 Qed.
+
+
+Section SEMICLOSED.
+
+  Definition semi_closed_timemap
+             (tm: TimeMap.t)
+             (mem: Memory.t)
+             (loc: Loc.t)
+             (ts: Time.t): Prop :=
+    forall l,
+      (exists from val released,
+          (<<GET: Memory.get l (tm l) mem = Some (from, Message.concrete val released)>>)) \/
+      (<<EQ: l = loc /\ tm l = ts>>)
+  .
+
+  Lemma closed_timemap_semi_closed tm mem loc ts
+        (CLOSED: Memory.closed_timemap tm mem)
+    :
+      semi_closed_timemap tm mem loc ts.
+  Proof.
+    ii. left. eauto.
+  Qed.
+
+  Lemma semi_closed_timemap_join tm0 tm1 mem loc ts
+        (CLOSED0: semi_closed_timemap tm0 mem loc ts)
+        (CLOSED1: semi_closed_timemap tm1 mem loc ts)
+    :
+      semi_closed_timemap (TimeMap.join tm0 tm1) mem loc ts.
+  Proof.
+    ii. specialize (CLOSED0 l). specialize (CLOSED1 l).
+    unfold TimeMap.join, Time.join. des; des_ifs; eauto.
+  Qed.
+
+  Lemma semi_closed_timemap_singleton mem loc ts
+        (INHABITED: Memory.inhabited mem)
+    :
+      semi_closed_timemap (TimeMap.singleton loc ts) mem loc ts.
+  Proof.
+    ii. unfold TimeMap.singleton.
+    destruct (Loc.eq_dec loc l).
+    - subst. right. split; auto. setoid_rewrite LocFun.add_spec_eq. auto.
+    - left. esplits. setoid_rewrite LocFun.add_spec_neq; eauto.
+  Qed.
+
+  Lemma semi_closed_timemap_add tm mem0 loc from ts val released mem1
+        (CLOSED: semi_closed_timemap tm mem0 loc ts)
+        (ADD: Memory.add mem0 loc from ts (Message.concrete val released) mem1)
+    :
+      Memory.closed_timemap tm mem1.
+  Proof.
+    ii. specialize (CLOSED loc0). des.
+    - esplits. eapply Memory.add_get1 in GET; eauto.
+    - subst. eapply Memory.add_get0 in ADD. des. eauto.
+  Qed.
+
+  Lemma semi_closed_timemap_split tm mem0 loc ts1 ts2 ts3 msg val released mem1
+        (CLOSED: semi_closed_timemap tm mem0 loc ts2)
+        (SPLIT: Memory.split mem0 loc ts1 ts2 ts3 (Message.concrete val released) msg mem1)
+    :
+      Memory.closed_timemap tm mem1.
+  Proof.
+    ii. specialize (CLOSED loc0). des.
+    - eapply Memory.split_get1 in GET; eauto. des. eauto.
+    - subst. eapply Memory.split_get0 in SPLIT. des. eauto.
+  Qed.
+
+  Lemma semi_closed_timemap_lower tm mem0 loc from to msg val released mem1
+        (CLOSED: semi_closed_timemap tm mem0 loc to)
+        (LOWER: Memory.lower mem0 loc from to msg (Message.concrete val released) mem1)
+    :
+      Memory.closed_timemap tm mem1.
+  Proof.
+    ii. specialize (CLOSED loc0). des.
+    - eapply Memory.lower_get1 in GET; eauto. des. inv MSG_LE. eauto.
+    - subst. eapply Memory.lower_get0 in LOWER. des. eauto.
+  Qed.
+
+  Lemma semi_closed_timemap_future tm mem0 loc ts mem1
+        (CLOSED: semi_closed_timemap tm mem0 loc ts)
+        (FUTURE: Memory.future_weak mem0 mem1)
+    :
+      semi_closed_timemap tm mem1 loc ts.
+  Proof.
+    ii. specialize (CLOSED l). des.
+    - eapply Memory.future_weak_get1 in GET; eauto. des.
+      inv MSG_LE. eauto.
+    - subst. eauto.
+  Qed.
+
+  Inductive semi_closed_view (view:View.t) (mem:Memory.t) (loc: Loc.t) (ts: Time.t): Prop :=
+  | semi_closed_view_intro
+      (PLN: semi_closed_timemap view.(View.pln) mem loc ts)
+      (RLX: semi_closed_timemap view.(View.rlx) mem loc ts)
+  .
+  Hint Constructors semi_closed_view.
+
+  Lemma closed_view_semi_closed vw mem loc ts
+        (CLOSED: Memory.closed_view vw mem)
+    :
+      semi_closed_view vw mem loc ts.
+  Proof.
+    inv CLOSED. econs.
+    - eapply closed_timemap_semi_closed; eauto.
+    - eapply closed_timemap_semi_closed; eauto.
+  Qed.
+
+  Lemma semi_closed_view_join vw0 vw1 mem loc ts
+        (CLOSED0: semi_closed_view vw0 mem loc ts)
+        (CLOSED1: semi_closed_view vw1 mem loc ts)
+    :
+      semi_closed_view (View.join vw0 vw1) mem loc ts.
+  Proof.
+    inv CLOSED0. inv CLOSED1. econs.
+    - eapply semi_closed_timemap_join; eauto.
+    - eapply semi_closed_timemap_join; eauto.
+  Qed.
+
+  Lemma semi_closed_view_singleton mem loc ts
+        (INHABITED: Memory.inhabited mem)
+    :
+      semi_closed_view (View.singleton_ur loc ts) mem loc ts.
+  Proof.
+    econs; ss.
+    - eapply semi_closed_timemap_singleton; eauto.
+    - eapply semi_closed_timemap_singleton; eauto.
+  Qed.
+
+  Lemma semi_closed_view_add vw mem0 loc from ts val released mem1
+        (CLOSED: semi_closed_view vw mem0 loc ts)
+        (ADD: Memory.add mem0 loc from ts (Message.concrete val released) mem1)
+    :
+      Memory.closed_view vw mem1.
+  Proof.
+    inv CLOSED. econs.
+    - eapply semi_closed_timemap_add; eauto.
+    - eapply semi_closed_timemap_add; eauto.
+  Qed.
+
+  Lemma semi_closed_view_split vw mem0 loc ts1 ts2 ts3 msg val released mem1
+        (CLOSED: semi_closed_view vw mem0 loc ts2)
+        (SPLIT: Memory.split mem0 loc ts1 ts2 ts3 (Message.concrete val released) msg mem1)
+    :
+      Memory.closed_view vw mem1.
+  Proof.
+    inv CLOSED. econs.
+    - eapply semi_closed_timemap_split; eauto.
+    - eapply semi_closed_timemap_split; eauto.
+  Qed.
+
+  Lemma semi_closed_view_lower vw mem0 loc from to msg val released mem1
+        (CLOSED: semi_closed_view vw mem0 loc to)
+        (LOWER: Memory.lower mem0 loc from to msg (Message.concrete val released) mem1)
+    :
+      Memory.closed_view vw mem1.
+  Proof.
+    inv CLOSED. econs.
+    - eapply semi_closed_timemap_lower; eauto.
+    - eapply semi_closed_timemap_lower; eauto.
+  Qed.
+
+  Lemma semi_closed_view_future vw mem0 loc ts mem1
+        (CLOSED: semi_closed_view vw mem0 loc ts)
+        (FUTURE: Memory.future_weak mem0 mem1)
+    :
+      semi_closed_view vw mem1 loc ts.
+  Proof.
+    inv CLOSED. econs.
+    - eapply semi_closed_timemap_future; eauto.
+    - eapply semi_closed_timemap_future; eauto.
+  Qed.
+
+  Inductive semi_closed_opt_view: forall (view:option View.t) (mem:Memory.t)
+                                         (loc: Loc.t) (ts: Time.t), Prop :=
+  | semi_closed_opt_view_some
+      view mem loc ts
+      (CLOSED: semi_closed_view view mem loc ts):
+      semi_closed_opt_view (Some view) mem loc ts
+  | semi_closed_opt_view_none
+      mem loc ts:
+      semi_closed_opt_view None mem loc ts
+  .
+  Hint Constructors semi_closed_opt_view.
+
+  Lemma closed_opt_view_semi_closed vw mem loc ts
+        (CLOSED: Memory.closed_opt_view vw mem)
+    :
+      semi_closed_opt_view vw mem loc ts.
+  Proof.
+    inv CLOSED; econs.
+    eapply closed_view_semi_closed; eauto.
+  Qed.
+
+  Lemma unwrap_closed_opt_view
+        view mem loc ts
+        (CLOSED: semi_closed_opt_view view mem loc ts)
+        (INHABITED: Memory.inhabited mem):
+    semi_closed_view view.(View.unwrap) mem loc ts.
+  Proof.
+    inv CLOSED; ss.
+    eapply closed_view_semi_closed. apply Memory.closed_view_bot. ss.
+  Qed.
+
+  Lemma semi_closed_opt_view_add vw mem0 loc from ts val released mem1
+        (CLOSED: semi_closed_opt_view vw mem0 loc ts)
+        (ADD: Memory.add mem0 loc from ts (Message.concrete val released) mem1)
+    :
+      Memory.closed_opt_view vw mem1.
+  Proof.
+    inv CLOSED; econs.
+    eapply semi_closed_view_add; eauto.
+  Qed.
+
+  Lemma semi_closed_opt_view_split vw mem0 loc ts1 ts2 ts3 msg val released mem1
+        (CLOSED: semi_closed_opt_view vw mem0 loc ts2)
+        (SPLIT: Memory.split mem0 loc ts1 ts2 ts3 (Message.concrete val released) msg mem1)
+    :
+      Memory.closed_opt_view vw mem1.
+  Proof.
+    inv CLOSED; econs.
+    eapply semi_closed_view_split; eauto.
+  Qed.
+
+  Lemma semi_closed_opt_view_lower vw mem0 loc from to msg val released mem1
+        (CLOSED: semi_closed_opt_view vw mem0 loc to)
+        (LOWER: Memory.lower mem0 loc from to msg (Message.concrete val released) mem1)
+    :
+      Memory.closed_opt_view vw mem1.
+  Proof.
+    inv CLOSED; econs.
+    eapply semi_closed_view_lower; eauto.
+  Qed.
+
+  Lemma semi_closed_opt_view_future vw mem0 loc ts mem1
+        (CLOSED: semi_closed_opt_view vw mem0 loc ts)
+        (FUTURE: Memory.future_weak mem0 mem1)
+    :
+      semi_closed_opt_view vw mem1 loc ts.
+  Proof.
+    inv CLOSED; econs.
+    eapply semi_closed_view_future; eauto.
+  Qed.
+
+  Inductive semi_closed_message: forall (msg:Message.t) (mem:Memory.t)
+                                        (loc: Loc.t) (ts: Time.t), Prop :=
+  | semi_closed_message_concrete
+      val released mem loc ts
+      (CLOSED: semi_closed_opt_view released mem loc ts):
+      semi_closed_message (Message.concrete val released) mem loc ts
+  | semi_closed_message_reserve
+      mem loc ts:
+      semi_closed_message Message.reserve mem loc ts
+  .
+  Hint Constructors semi_closed_message.
+
+  Lemma closed_message_semi_closed msg mem loc ts
+        (CLOSED: Memory.closed_message msg mem)
+    :
+      semi_closed_message msg mem loc ts.
+  Proof.
+    inv CLOSED; econs. eapply closed_opt_view_semi_closed; eauto.
+  Qed.
+
+  Lemma semi_closed_message_add vw mem0 loc from ts val released mem1
+        (CLOSED: semi_closed_message vw mem0 loc ts)
+        (ADD: Memory.add mem0 loc from ts (Message.concrete val released) mem1)
+    :
+      Memory.closed_message vw mem1.
+  Proof.
+    inv CLOSED; econs.
+    eapply semi_closed_opt_view_add; eauto.
+  Qed.
+
+  Lemma semi_closed_message_split vw mem0 loc ts1 ts2 ts3 msg val released mem1
+        (CLOSED: semi_closed_message vw mem0 loc ts2)
+        (SPLIT: Memory.split mem0 loc ts1 ts2 ts3 (Message.concrete val released) msg mem1)
+    :
+      Memory.closed_message vw mem1.
+  Proof.
+    inv CLOSED; econs.
+    eapply semi_closed_opt_view_split; eauto.
+  Qed.
+
+  Lemma semi_closed_message_lower vw mem0 loc from to msg val released mem1
+        (CLOSED: semi_closed_message vw mem0 loc to)
+        (LOWER: Memory.lower mem0 loc from to msg (Message.concrete val released) mem1)
+    :
+      Memory.closed_message vw mem1.
+  Proof.
+    inv CLOSED; econs.
+    eapply semi_closed_opt_view_lower; eauto.
+  Qed.
+
+  Lemma semi_closed_message_future vw mem0 loc ts mem1
+        (CLOSED: semi_closed_message vw mem0 loc ts)
+        (FUTURE: Memory.future_weak mem0 mem1)
+    :
+      semi_closed_message vw mem1 loc ts.
+  Proof.
+    inv CLOSED; econs.
+    eapply semi_closed_opt_view_future; eauto.
+  Qed.
+
+End SEMICLOSED.
